restruct and simplify

Protocol/Crypto.fst
@@ -4,21 +4,15 @@ open Protocol
 type prin = string
 type pubkey :: prin => *
 type privkey :: prin => *
-type dsig = string
-type nonce = string
-
-(*type pubkey :: * => * =
-    | PublicKey :  prin -> pubkey prin
-*)
+type dsig
+type nonce
+type cypher
 
 (*Verification*)
 type Log :: prin => string => E
 
 val Keygen:  p:prin
           -> (pubkey p * privkey p)
-(*let Keygen prin =
-    let (pk,sk) = KeyGenExt prin in
-    (PublicKey pk,privkey sk)*)
 
 val Sign:  p:prin
         -> privkey p
@@ -31,17 +25,23 @@ val VerifySignature: p:prin
         -> dsig
         -> b:bool{b=true ==> Log p msg}
 
+
+val Encrypt: p:prin
+        -> pubkey p
+        -> msg:string{Log p msg}
+        -> cypher
+
+val Decrypt: p:prin
+        -> p privkey
+        -> cypher
+        -> msg:string
+
+val GenerateNonce: prin -> nonce (*Add refinement to ensure unqueness*)
+
 val AuthenticateUser: user:string
         -> password:string
         -> challenge:nonce 
         -> b:bool{b=true ==> Log user challenge}
-
-val GenerateNonce: prin -> nonce (*Add refinement to ensure unqueness*)
-(*val Encrypt: ...
-
-val Decrypt: ...*)
-
-
 
 
 (*Crypto functions*)
