Protocol/ServiceProvider.fst
@@ -1,41 +1,32 @@
 module Serviceprovider
 
-open Lib
-open SessionManager
-open ContentServer
-open Protocol
-open Saml
+open SamlProtocol
 open Crypto
-open Network
+
+
 
 val serviceprovider:  me:prin -> pubkey me -> privkey me ->
-                      browser:prin -> idp:prin -> pubkey idp -> unit 
-let serviceprovider me pubk privk browser idp pubkidp = 
-  let req = Recieve browser in (*1*) (*7*)
-  match req with
-  | Get (uri,params,cookies) -> 
+                      client:prin -> idp:prin -> pubkey idp -> unit 
+let serviceprovider me pubk privk client idp pubkidp = 
+ let req = ReceiveSaml client in
+ match req with
+  | Login (url) -> (*Create AuthnRequest and send back*)
+    let authnReq = CreateAuthnRequestMessage me idp in
+    assume(Log me authnReq) (*Protocol event*);
+    let sigSP = Sign me privk authnReq in
+    let resp = AuthnRequest me idp authnReq sigSP in 
+    SendSaml client resp; (*2*)
+    serviceprovider me pubk privk client idp pubkidp (*Start over*)
 
-    (*Check for valid session*)
-    if hasValidSession cookies then
-      let resp = Response (getContent uri) [] in
-      Send resp (*8*)
-    else (*Create AuthnRequest and send (via client) to idp*)
-      (let authnReq = CreateAuthnRequest me idp in 
-      assume(Log me authnReq) (*Protocol event*);
-      let sigSP = Sign me privk authnReq in
-      let samlMsg = SamlAuthnRequestMessage authnReq sigSP in
-      let resp = CreateRedirectResponse idp samlMsg in 
-      Send resp (*2*))
-
-  | Post (uri, qparams, fparams, cookies) -> 
-      let msg = getStrInTupleList fparams "SamlMessage" in
-      let sigIDP = getStrInTupleList fparams "Signature" in
-      if VerifySignature idp pubkidp msg sigIDP
+  | AuthResponseMessage (issuer, destination, assertion) -> 
+    match assertion with
+    | SignedAssertion (token,sigIDP) ->
+      if VerifySignature idp pubkidp token sigIDP
       then
-        (assert(Log idp msg);
-          let ak =  GenerateNonce me in
-          let resp = Response (getContent "Logged-in") [("AuthenticationKey", ak)] in
-          Send resp) (*8*)
-      else Send (ErrorResponse 403 (getErrorPage 403) [])(*8.1*)
-  
-  | _ -> Send (ErrorResponse 400 (getErrorPage 400) [])
+        (assert(Log idp token);
+        let resp = LoginResponse "You are now logged in" in
+        SendSaml client resp) (*8*)
+      else SendSaml client (Failed 403);(*8.1*)
+      serviceprovider me pubk privk client idp pubkidp (*Start over*)
+  | _ -> SendSaml client (Failed 400);(*8.1*)
+        serviceprovider me pubk privk client idp pubkidp (*Start over*)
