Protocol/identityprovider.fst
@@ -1,70 +1,23 @@
 module Identityprovider
 
-open Lib
-open SessionManager
-open Protocol
-open Saml
+open SamlProtocol
 open Crypto
-open Network
-open ContentServer
-
-(*TODO: 
-  - Make it compile
-  - Encrypt/decrypt
-  - Ensure it follows model*)
-
-let CheckSessionAndBuildResponse me privk authReq browser serviceprovider pubksp cookies = 
-        if hasValidSession cookies then
-          let subject = GetSessionSubject cookies in
-          let assertion = IssueSamlAssertion me privk authReq subject serviceprovider pubksp in
-          let resp = CreateSamlResponse me authReq assertion in
-          resp
-
-        else
-          let challenge = GenerateNonce me in
-          let challengeMessage = CreateChallengeMessage me challenge in
-          challengeMessage (*4*)
-
-let HandleGetResponse msg me privk browser serviceprovider pubksp cookies =
-match msg with 
-    | SamlAuthnRequestMessage (authReq, sigSP) ->
-      if (VerifySignature serviceprovider pubksp authReq sigSP) then
-        (assert (Log serviceprovider authReq);
-        CheckSessionAndBuildResponse me privk authReq browser serviceprovider pubksp cookies)
-       
-      else ErrorResponse 403 (getErrorPage 403) [] (*4.1*) (*TODO*)
-    | _ -> ErrorResponse 403 (getErrorPage 403) [] (*4.1*) (*TODO*)
-
-let HandlePostResponse = ()
-    (*Check credentials and challenge
-    if AuthenticateUser user password challenge'
-    then
-      (assert (Log2 user password challenge');
-
-      let samlresponse = CreateSamlResponse me serviceprovider Success in
-      assume(Log me samlresponse);
-      let sigIDP = Sign me privk samlresponse in 
-      let response = SamlProtocolMessage serviceprovider samlresponse sigIDP in
-      Send browser response(*6*))
-    else Send browser (Failed (400))(*6.3*)*)
-
 
 val identityprovider: me:prin -> pubkey me -> privkey me 
-                      -> browser:prin -> sp:prin -> pubkey sp
+                      -> client:prin -> sp:prin -> pubkey sp
                       -> unit
-let identityprovider me pubk privk browser serviceprovider pubksp =
-	let req = Recieve browser in (*3 & 11*)
+let identityprovider me pubk privk client serviceprovider pubksp =
+	let req = ReceiveSaml client in (*3 & 11*)
 	match req with
-	| Get (uri, params, cookies) ->
-    let msg = GetSamlMessage params in
-    let resp = HandleGetResponse msg me pubk privk browser serviceprovider pubksp in
-    Send browser resp
-
-  | Post (uri, qparams, fparams, cookies) -> 
-    let params = append qparams fparams in
-    let msg = GetSamlMessage params in
-    let resp = HandlePostResponse msg in
-    Send browser resp    
-
-  | _ -> Send (ErrorResponse 400 (getErrorPage 400) [])
+	| AuthnRequest (issuer, destination, message, sigSP) ->
+    if (VerifySignature serviceprovider pubksp message sigSP) then
+      (assert (Log serviceprovider message);
+      let challenge = GenerateNonce me in
+      let resp = UserCredRequest challenge in
+      SendSaml client resp;
+      identityprovider me pubk privk client serviceprovider pubksp (*Start over*))
+    else
+      SendSaml client (Failed 400)(*8.1*)
+  | _ -> SendSaml client (Failed 400);(*8.1*)
+        identityprovider me pubk privk client serviceprovider pubksp (*Start over*)
 
