Protocol/experiments/ServiceProvider.fst
@@ -1,0 +1,41 @@
+module Serviceprovider
+
+open Lib
+open SessionManager
+open ContentServer
+open Protocol
+open Saml
+open Crypto
+open Network
+
+val serviceprovider:  me:prin -> pubkey me -> privkey me ->
+                      browser:prin -> idp:prin -> pubkey idp -> unit 
+let serviceprovider me pubk privk browser idp pubkidp = 
+  let req = Recieve browser in (*1*) (*7*)
+  match req with
+  | Get (uri,params,cookies) -> 
+
+    (*Check for valid session*)
+    if hasValidSession cookies then
+      let resp = Response (getContent uri) [] in
+      Send resp (*8*)
+    else (*Create AuthnRequest and send (via client) to idp*)
+      (let authnReq = CreateAuthnRequest me idp in 
+      assume(Log me authnReq) (*Protocol event*);
+      let sigSP = Sign me privk authnReq in
+      let samlMsg = SamlAuthnRequestMessage authnReq sigSP in
+      let resp = CreateRedirectResponse idp samlMsg in 
+      Send resp (*2*))
+
+  | Post (uri, qparams, fparams, cookies) -> 
+      let msg = getStrInTupleList fparams "SamlMessage" in
+      let sigIDP = getStrInTupleList fparams "Signature" in
+      if VerifySignature idp pubkidp msg sigIDP
+      then
+        (assert(Log idp msg);
+          let ak =  GenerateNonce me in
+          let resp = Response (getContent "Logged-in") [("AuthenticationKey", ak)] in
+          Send resp) (*8*)
+      else Send (ErrorResponse 403 (getErrorPage 403) [])(*8.1*)
+  
+  | _ -> Send (ErrorResponse 400 (getErrorPage 400) [])
