Protocol/experiments/identityprovider.fst
@@ -1,0 +1,70 @@
+module Identityprovider
+
+open Lib
+open SessionManager
+open Protocol
+open Saml
+open Crypto
+open Network
+open ContentServer
+
+(*TODO: 
+  - Make it compile
+  - Encrypt/decrypt
+  - Ensure it follows model*)
+
+let CheckSessionAndBuildResponse me privk authReq browser serviceprovider pubksp cookies = 
+        if hasValidSession cookies then
+          let subject = GetSessionSubject cookies in
+          let assertion = IssueSamlAssertion me privk authReq subject serviceprovider pubksp in
+          let resp = CreateSamlResponse me authReq assertion in
+          resp
+
+        else
+          let challenge = GenerateNonce me in
+          let challengeMessage = CreateChallengeMessage me challenge in
+          challengeMessage (*4*)
+
+let HandleGetResponse msg me privk browser serviceprovider pubksp cookies =
+match msg with 
+    | SamlAuthnRequestMessage (authReq, sigSP) ->
+      if (VerifySignature serviceprovider pubksp authReq sigSP) then
+        (assert (Log serviceprovider authReq);
+        CheckSessionAndBuildResponse me privk authReq browser serviceprovider pubksp cookies)
+       
+      else ErrorResponse 403 (getErrorPage 403) [] (*4.1*) (*TODO*)
+    | _ -> ErrorResponse 403 (getErrorPage 403) [] (*4.1*) (*TODO*)
+
+let HandlePostResponse = ()
+    (*Check credentials and challenge
+    if AuthenticateUser user password challenge'
+    then
+      (assert (Log2 user password challenge');
+
+      let samlresponse = CreateSamlResponse me serviceprovider Success in
+      assume(Log me samlresponse);
+      let sigIDP = Sign me privk samlresponse in 
+      let response = SamlProtocolMessage serviceprovider samlresponse sigIDP in
+      Send browser response(*6*))
+    else Send browser (Failed (400))(*6.3*)*)
+
+
+val identityprovider: me:prin -> pubkey me -> privkey me 
+                      -> browser:prin -> sp:prin -> pubkey sp
+                      -> unit
+let identityprovider me pubk privk browser serviceprovider pubksp =
+	let req = Recieve browser in (*3 & 11*)
+	match req with
+	| Get (uri, params, cookies) ->
+    let msg = GetSamlMessage params in
+    let resp = HandleGetResponse msg me pubk privk browser serviceprovider pubksp in
+    Send browser resp
+
+  | Post (uri, qparams, fparams, cookies) -> 
+    let params = append qparams fparams in
+    let msg = GetSamlMessage params in
+    let resp = HandlePostResponse msg in
+    Send browser resp    
+
+  | _ -> Send (ErrorResponse 400 (getErrorPage 400) [])
+
