Protocol/main.fst
@@ -1,15 +1,15 @@
 module Main
 
-open Protocol
-open Browser
+open SamlProtocol
+open Crypto
 open Serviceprovider
 open Identityprovider
-open ModelUtil
+
+val Fork: list (unit -> unit) -> unit
 
 let main attacker =
 	let sppk, spsk = Keygen "https://serviceprovider.org" in 
 	let idppk, idpsk = Keygen "https://identityprovider.org" in 
 	Fork [	attacker;
-		(fun () -> browser "browser" "https://serviceprovider.org/protectedresource" "me" "myPassword");
 		(fun () -> serviceprovider "https://serviceprovider.org" sppk spsk "browser" "https://identityprovider.org" idppk);
 		(fun () -> identityprovider "https://identityprovider.org" idppk idpsk "browser" "https://serviceprovider.org" sppk)]
