Protocol/report-examples/hello.fst
@@ -1,0 +1,5 @@
+module hello
+
+let _ = 
+	let x:string = "hello world" in
+	print_string x
