Protocol/report-examples/refinements.fst
@@ -1,0 +1,7 @@
+module X
+
+(* Declare a type pos of positive numbers *)
+type pos = i:int{i>0}
+
+let x:pos = 1
+let y:pos = 0 (* Will not type-check*)
