Protocol/serviceprovicer-example/serviceprovider.fst
@@ -1,0 +1,62 @@
+module Crypto
+
+type prin = string
+type pubkey :: prin => *
+type privkey :: prin => *
+type dsig
+
+(*Verification*)
+type Log :: prin => string => E
+
+val Keygen:  p:prin
+          -> (pubkey p * privkey p)
+
+val Sign:  p:prin
+        -> privkey p
+        -> msg:string{Log p msg}
+        -> dsig
+
+val VerifySignature: p:prin
+        -> pubkey p 
+        -> msg:string
+        -> dsig
+        -> b:bool{b=true ==> Log p msg}
+end
+
+
+
+module SamlProtocol
+
+open Crypto
+
+type uri
+
+type SamlMessage =
+  | Login: uri -> SamlMessage
+  | AuthnRequest: issuer:prin ->  destination:prin -> message:string -> dsig -> SamlMessage
+  | Failed: int -> SamlMessage
+
+val SendSaml: prin -> SamlMessage -> unit
+val ReceiveSaml: prin -> SamlMessage 
+
+val CreateAuthnRequestMessage: issuer:prin -> destination:prin -> string
+
+end
+
+module Serviceprovider
+
+open Crypto
+open SamlProtocol
+
+val serviceprovider:  me:prin -> pubkey me -> privkey me ->
+                      client:prin -> idp:prin -> pubkey idp -> unit 
+let serviceprovider me pubk privk client idp pubkidp = 
+ let req = ReceiveSaml client in (*1*)
+ match req with
+  | Login (url) -> 
+    let authnReq = CreateAuthnRequestMessage me idp in
+    assume(Log me authnReq);
+    let sigSP = Sign me privk authnReq in
+    let resp = AuthnRequest me idp authnReq sigSP in 
+    SendSaml client resp (*2*)
+  | _ -> SendSaml client (Failed 400)(*2.1*)
